stuff

Ack.lean
@@ -1,10 +1,20 @@
+private def Nat.rec' {motive : Nat → Sort u} (zero : motive zero) (succ : ∀ n, motive n → motive (succ n)) : ∀ n, motive n
+  | .zero => zero
+  | .succ n => succ n (rec' zero succ n)
+
+@[csimp]
+private theorem Nat.rec_eq_rec' : @rec = @rec' := by
+  funext motive zero succ n
+  induction n with
+  | zero => rfl
+  | succ n ih => exact congrArg (succ n) ih
+
 def ack : Nat → Nat → Nat
   | 0, n => n + 1
   | m + 1, 0 => ack m 1
   | m + 1, n + 1 => ack m (ack (m + 1) n)
 termination_by _ m n => (m, n)
 
-noncomputable
 def ack' : Nat → Nat → Nat :=
   Nat.rec
     (λ n => n + 1)
