Abt.lean
@@ -1,0 +1,740 @@
+import Lean
+
+def Fin.zero : Fin (.succ n) :=
+  ⟨0, n.zero_lt_succ⟩
+
+def Fin.last : Fin (.succ n) :=
+  ⟨n, n.lt_succ_self⟩
+
+def Fin.castSucc : Fin n → Fin n.succ
+  | ⟨i, h⟩ => ⟨i, .step h⟩
+
+def String.joinSep l sep := join (List.intersperse sep l)
+
+open Lean in
+elab tk:"#print " "instances " t:term : command =>
+  Elab.Command.runTermElabM λ _ => do
+    let e ← Elab.Term.elabType t
+    let insts ← Meta.SynthInstance.getInstances e
+    let insts ← insts.mapM λ inst => return m!"{inst} : {← Meta.inferType inst}"
+    logInfoAt tk <| .joinSep insts.toList Format.line
+
+/-
+def Fin.cast (h' : k ≤ n) : Fin k → Fin n
+  | ⟨i, h⟩ => ⟨i, Nat.le_trans h h'⟩
+
+def Fin.cases {α : Fin (n + 1) → Sort u} (zero : α .zero) (succ : ∀ i, α (Fin.succ i)) : ∀ i, α i
+  | ⟨0, _⟩ => zero
+  | ⟨i + 1, h⟩ => succ ⟨i, Nat.pred_le_pred h⟩
+
+def Fin.revCases {α : Fin (n + 1) → Sort u} (last : α .last) (castSucc : ∀ i, α (Fin.castSucc i)) : ∀ i, α i
+  | ⟨i, h⟩ =>
+    if h' : i = n
+    then by simp [h']; exact last
+    else castSucc ⟨i, Nat.lt_of_le_of_ne (Nat.pred_le_pred h) h'⟩
+
+namespace FinTuple
+
+def foldr' {α : Fin n → Sort u} (f : ∀ {i}, Nat → α i → β → β) (y : β) (xs : ∀ i, α i) : β :=
+  foldr (λ x (y, k) => (f k x y, k + 1)) (y, 0) xs |>.1
+
+def foldl {α : Fin n → Sort u} (f : ∀ {i}, β → α i → β) (y : β) (xs : ∀ i, α i) : β :=
+  match n with
+  | 0 => y
+  | _ + 1 => foldl f (f y (xs .zero)) (xs ·.succ)
+
+def dfoldr {α : Fin n → Sort u} {β : Fin (n + 1) → Sort v} (f : ∀ {i}, α i → β i.succ → β i.castSucc) (y : β .last) (xs : ∀ i, α i) : β .zero :=
+  match n with
+  | 0 => y
+  | _ + 1 => f (xs .zero) (dfoldr (β := β ∘ .succ) f y (xs ·.succ))
+
+def dfoldl {α : Fin n → Sort u} {β : Fin (n + 1) → Sort v} (f : ∀ {i}, β i.castSucc → α i → β i.succ) (y : β .zero) (xs : ∀ i, α i) : β .last :=
+  match n with
+  | 0 => y
+  | _ + 1 => dfoldl (β := β ∘ .succ) (f ·) (f (i := .zero) y (xs .zero)) (xs ·.succ)
+
+def toStringAux : ∀ {n} {α : Fin n → Type u} [∀ i, ToString (α i)], Bool → (∀ i, α i) → String
+  | 0, _, _, _, _ => ""
+  | _ + 1, _, _, true, xs => toString (xs 0) ++ toStringAux false (xs ·.succ)
+  | _ + 1, _, _, false, xs => ", " ++ toString (xs 0) ++ toStringAux false (xs ·.succ)
+
+instance {α : Fin n → Type u} [∀ i, ToString (α i)] : ToString (∀ i, α i) where
+  toString xs := "⟦" ++ toStringAux true xs ++ "⟧"
+
+macro "⟦" t:term,* "⟧'" : term => `(@Sigma.mk Nat ((_ : Fin ·) → _) _ ⟦$t,*⟧)
+
+end FinTuple
+-/
+
+namespace FinTuple
+
+def nil {α : Fin 0 → Sort u} i : α i := nomatch i
+
+def cons {α : Fin (.succ n) → Sort u} (x : α .zero) (xs : ∀ i, α (.succ i)) : ∀ i, α i
+  | ⟨0, _⟩ => x
+  | ⟨i + 1, h⟩ => xs ⟨i, Nat.lt_of_succ_lt_succ h⟩
+
+scoped syntax "⟦" term,* "⟧" : term
+
+macro_rules
+  | `(⟦⟧)          => ``(nil)
+  | `(⟦$x⟧)        => ``(cons $x ⟦⟧)
+  | `(⟦$x, $xs,*⟧) => ``(cons $x ⟦$xs,*⟧)
+
+@[app_unexpander nil]
+protected def nilUnexpander : Lean.PrettyPrinter.Unexpander
+  | `($_:ident) => ``(⟦⟧)
+  | _           => throw ()
+
+@[app_unexpander cons]
+protected def consUnexpander : Lean.PrettyPrinter.Unexpander
+  | `($_ $x ⟦⟧)      => ``(⟦$x⟧)
+  | `($_ $x ⟦$xs,*⟧) => ``(⟦$x, $xs,*⟧)
+  | _                => throw ()
+
+def foldr {α : Fin n → Sort u} {β : Sort v} (f : ∀ {i}, α i → β → β) (y : β) (xs : ∀ i, α i) : β :=
+  match n with
+  | 0 => y
+  | _ + 1 => f (xs .zero) (foldr f y (xs ·.succ))
+
+def toList : (Fin n → α) → List α :=
+  foldr .cons .nil
+
+end FinTuple
+
+variable {α : Type u} (β : α → Sort v) in
+inductive DList : List α → Sort _
+  | nil : DList []
+  | cons : β a → DList as → DList (a :: as)
+
+namespace DList
+
+scoped syntax "⟦" term,* "⟧" : term
+
+macro_rules
+  | `(⟦⟧)          => ``(nil)
+  | `(⟦$x⟧)        => ``(cons $x ⟦⟧)
+  | `(⟦$x, $xs,*⟧) => ``(cons $x ⟦$xs,*⟧)
+
+@[app_unexpander nil]
+protected def nilUnexpander : Lean.PrettyPrinter.Unexpander
+  | `($_) => ``(⟦⟧)
+
+@[app_unexpander cons]
+protected def consUnexpander : Lean.PrettyPrinter.Unexpander
+  | `($_ $x ⟦⟧)      => ``(⟦$x⟧)
+  | `($_ $x ⟦$xs,*⟧) => ``(⟦$x, $xs,*⟧)
+  | _                => throw ()
+
+variable {α : Type u} {β₁ : α → Type v₁} {β₂ : α → Type v₂} (f : ∀ {a}, β₁ a → β₂ a) in
+def map : DList β₁ as → DList β₂ as
+  | nil => nil
+  | cons x xs => cons (f x) (map xs)
+
+variable {α : Type u} {β : α → Sort v} {γ : Sort w} (f : ∀ {a}, β a → γ → γ) (y : γ) in
+def foldr : DList β as → γ
+  | nil => y
+  | cons x xs => f x (foldr xs)
+
+def toList : DList (λ _ => α) as → List α
+  | nil => []
+  | cons x xs => x :: toList xs
+
+universe w in
+variable
+  {α : Type u}
+  {β : α → Sort v}
+  {motive : ∀ as, DList β as → Sort w}
+  (nil : motive [] nil)
+  (cons : ∀ {a as} x xs, motive as xs → motive (a :: as) (cons x xs))
+in
+private def rec' : ∀ t, motive as t
+  | .nil => nil
+  | .cons x xs => cons x xs (rec' xs)
+
+@[csimp]
+private theorem rec_eq_rec' : @rec = @rec' := by
+  funext α β motive nil cons as t
+  induction t with
+  | nil => rfl
+  | cons x xs ih => exact congrArg _ ih
+
+end DList
+
+structure Var (s : α) where
+  x : Nat
+
+instance : DecidableEq (Var s)
+  | ⟨x⟩, ⟨y⟩ =>
+    if h : x = y
+    then isTrue (congrArg Var.mk h)
+    else isFalse (h ∘ congrArg Var.x)
+
+instance : OfNat (Var s) n := ⟨⟨n⟩⟩
+
+protected partial def Var.toString : Var s → String
+  | ⟨x⟩ => ⟨f x []⟩
+where f x s :=
+  let s := Char.ofNat ('a'.toNat + x % 26) :: s
+  match x / 26 with
+  | 0 => s
+  | q + 1 => f q s
+
+instance : ToString (Var s) := ⟨Var.toString⟩
+
+instance : Coe String (Var s) where
+  coe s := ⟨s.foldl (λ x c => (x + 1) * 26 + (c.toNat - 'a'.toNat).min 25) 0 - 26 ^ s.length⟩
+
+/-
+syntax "ast " ident " where " (ident (" | " ident term*)*)* : command
+macro_rules
+  | `(ast $l where $[$s $[| $o $[$a]*]*]*) => do
+    let is ← (s.zip (o.zip a)).mapM λ (s, (o, a)) =>
+      `(inductive $s)
+    `(namespace $l $(⟨Lean.mkNullNode is⟩) end $l)
+
+set_option trace.Elab.command true in
+ast Example where
+  Exp
+  | var Var
+  | num "[" Nat "]"
+  | plus "(" Exp "; " Exp ")"
+  | times "(" Exp "; " Exp ")"
+-/
+
+namespace Example
+
+inductive Exp
+  | var : Var Exp → Exp
+  | num : Nat → Exp
+  | plus : Exp → Exp → Exp
+  | times : Exp → Exp → Exp
+
+instance : ToString Exp where
+  toString := f
+where f
+  | .var x => x.toString
+  | .num n => s!"num[{n}]"
+  | .plus e₁ e₂ => s!"plus({f e₁}; {f e₂})"
+  | .times e₁ e₂ => s!"times({f e₁}; {f e₂})"
+
+namespace Exp
+
+variable (e : Exp) (x : Var Exp) in
+def substExp : Exp → Exp
+  | var y => if y = x then e else .var y
+  | num n => num n
+  | plus e₁ e₂ => plus (substExp e₁) (substExp e₂)
+  | times e₁ e₂ => times (substExp e₁) (substExp e₂)
+
+#eval plus (num 2) (times (num 3) (var 0))
+#eval substExp (num 2) 0 (plus (var 0) (num 3))
+
+end Exp
+
+end Example
+
+variable {S : Type} (O : List S → S → Type) in
+inductive Ast : S → Type
+  | var (x : Var s) : Ast s
+  | op (o : O si s) (ai : DList Ast si) : Ast s
+
+namespace Ast
+
+section rec
+
+variable
+  {motive₁ : (s : S) → Ast O s → Sort u}
+  {motive₂ : ∀ si, DList (Ast O) si → Sort u}
+  (var : ∀ {s} x, motive₁ s (var x))
+  (op : ∀ {si s} o ai, motive₂ si ai → motive₁ s (op o ai))
+  (nil : motive₂ .nil .nil)
+  (cons : ∀ {s si} a ai, motive₁ s a → motive₂ si ai → motive₂ (.cons s si) (.cons a ai))
+
+mutual
+
+private def rec' : ∀ a, motive₁ s a
+  | .var x => var x
+  | .op o ai => op o ai (rec_1' ai)
+
+private def rec_1' : ∀ ai, motive₂ si ai
+  | .nil => nil
+  | .cons a ai => cons a ai (rec' a) (rec_1' ai)
+
+end
+
+mutual
+
+private theorem rec_eq_rec'_ : ∀ a, @rec S O motive₁ motive₂ @var @op @nil @cons s a = @rec' S O motive₁ motive₂ @var @op @nil @cons s a
+  | .var x => by unfold rec'; rfl
+  | .op o ai => by unfold rec'; exact congrArg (op o ai) (rec_1_eq_rec_1'_ ai)
+
+private theorem rec_1_eq_rec_1'_ : ∀ ai, @rec_1 S O motive₁ motive₂ @var @op @nil @cons si ai = @rec_1' S O motive₁ motive₂ @var @op @nil @cons si ai
+  | .nil => by unfold rec_1'; rfl
+  | .cons a ai => by unfold rec_1'; exact congr (congrArg (cons a ai) (rec_eq_rec'_ a)) (rec_1_eq_rec_1'_ ai)
+
+end
+
+end rec
+
+@[csimp]
+private theorem rec_eq_rec' : @rec = @rec' := by
+  funext S O motive₁ motive₂ var op nil cons s a
+  apply rec_eq_rec'_
+
+@[csimp]
+private theorem rec_1_eq_rec_1' : @rec_1 = @rec_1' := by
+  funext S O motive₁ motive₂ var op nil cons si ai
+  apply rec_1_eq_rec_1'_
+
+def ndrec
+  {motive : S → Type u}
+  (var : ∀ {s}, Var s → motive s)
+  (op : ∀ {si s}, O si s → DList (Ast O) si → DList motive si → motive s)
+: ∀ {a}, Ast O a → motive a :=
+  @rec S O (λ s _ => motive s) (λ si _ => DList motive si) var op DList.nil λ _ _ => DList.cons
+
+def subst [DecidableEq S] {s : S} (a : Ast O s) (x : Var s) : Ast O t → Ast O t :=
+  ndrec
+    (λ {t} y => if h : t = s then if h ▸ y = x then h ▸ a else var y else var y)
+    (λ o _ai ai' => op o ai')
+
+protected def toString [∀ si s, ToString (O si s)] : Ast O s → String :=
+  ndrec
+    (λ x => x.toString)
+    (λ | o, .nil, _ => toString o
+       | o, _, ai' => toString o ++ "(" ++ .joinSep ai'.toList "; " ++ ")")
+
+instance [∀ si s, ToString (O si s)] : ToString (Ast O s) := ⟨Ast.toString⟩
+
+end Ast
+
+variable {S : Type} (O : ∀ ⦃n⦄, (Fin n → S) → S → Type) in
+inductive Ast' : S → Type
+  | var (x : Var s) : Ast' s
+  | op {si : Fin n → S} (o : O si s) (ai : ∀ i, Ast' (si i)) : Ast' s
+
+namespace Ast'
+
+variable [DecidableEq S] {s : S} (a : Ast' O s) (x : Var s) in
+def subst : Ast' O t → Ast' O t
+  | var y => if h : t = s then if h ▸ y = x then h ▸ a else var y else var y
+  | op o ai => op o λ i => subst (ai i)
+
+protected def toString [∀ {n} si s, ToString (@O n si s)] : Ast' O s → String
+  | var x => x.toString
+  | op (n := 0) o _ => toString o
+  | op o ai => toString o ++ "(" ++ .joinSep (FinTuple.toList λ i => (ai i).toString) "; " ++ ")"
+
+instance [∀ {n} si s, ToString (@O n si s)] : ToString (Ast' O s) := ⟨Ast'.toString⟩
+
+end Ast'
+
+namespace ExampleAst
+
+open DList
+
+inductive S
+  | Exp
+deriving DecidableEq
+
+inductive O : List S → S → Type
+  | num : Nat → O [] .Exp
+  | plus : O [.Exp, .Exp] .Exp
+  | times : O [.Exp, .Exp] .Exp
+
+instance : ToString (O si s) where
+  toString
+    | .num n => s!"num[{n}]"
+    | .plus => "plus"
+    | .times => "times"
+
+abbrev Ast := _root_.Ast O
+
+abbrev Exp := Ast .Exp
+
+namespace Exp
+
+def var (x : Var S.Exp) : Exp := .var x
+def num (n : Nat) : Exp := .op (.num n) ⟦⟧
+def plus (a b : Exp) : Exp := .op .plus ⟦a, b⟧
+def times (a b : Exp) : Exp := .op .times ⟦a, b⟧
+
+#eval plus (num 2) (times (num 3) (var 0))
+#eval Ast.subst (num 2) 0 (plus (var 0) (num 3))
+
+end Exp
+
+end ExampleAst
+
+namespace ExampleAst'
+
+open FinTuple
+
+inductive S
+  | Exp
+deriving DecidableEq
+
+inductive O : ∀ ⦃n⦄, (Fin n → S) → S → Type
+  | num : Nat → O ⟦⟧ .Exp
+  | plus : O ⟦.Exp, .Exp⟧ .Exp
+  | times : O ⟦.Exp, .Exp⟧ .Exp
+
+instance : ToString (O si s) where
+  toString
+    | .num n => s!"num[{n}]"
+    | .plus => "plus"
+    | .times => "times"
+
+abbrev Ast := _root_.Ast' O
+
+abbrev Exp := Ast .Exp
+
+namespace Exp
+
+def var (x : Var S.Exp) : Exp := .var x
+def num (n : Nat) : Exp := .op (.num n) ⟦⟧
+def plus (a b : Exp) : Exp := .op .plus ⟦a, b⟧
+def times (a b : Exp) : Exp := .op .times ⟦a, b⟧
+
+#eval plus (num 2) (times (num 3) (var 0))
+#eval Ast'.subst (num 2) 0 (plus (var 0) (num 3))
+
+end Exp
+
+end ExampleAst'
+
+variable {S : Type} (O : List (List S × S) → S → Type) in
+inductive Abt₁ : S → Type
+  | bvar s (n : Nat) : Abt₁ s
+  | var (x : Var s) : Abt₁ s
+  | op (o : O si s) (ai : DList (Abt₁ ·.2) si) : Abt₁ s
+
+namespace Abt₁
+
+section rec
+
+variable
+  {motive₁ : (s : S) → Abt₁ O s → Sort u}
+  {motive₂ : (si : List (_ × S)) → DList (Abt₁ O ·.2) si → Sort u}
+  (bvar : ∀ s n, motive₁ s (bvar s n))
+  (var : ∀ {s} x, motive₁ s (var x))
+  (op : ∀ {si s} o ai, motive₂ si ai → motive₁ s (op o ai))
+  (nil : motive₂ .nil .nil)
+  (cons : ∀ {s si} a (ai : DList (Abt₁ O ·.2) si), motive₁ s.2 a → motive₂ si ai → motive₂ (.cons s si) (.cons a ai))
+
+mutual
+
+private def rec' : ∀ a, motive₁ s a
+  | .bvar s n => bvar s n
+  | .var x => var x
+  | .op o ai => op o ai (rec_1' ai)
+
+private def rec_1' : ∀ ai, motive₂ si ai
+  | .nil => nil
+  | .cons a ai => cons a ai (rec' a) (rec_1' ai)
+
+end
+
+mutual
+
+private theorem rec_eq_rec'_ : ∀ a, @rec S O motive₁ motive₂ @bvar @var @op @nil @cons s a = @rec' S O motive₁ motive₂ @bvar @var @op @nil @cons s a
+  | .bvar s n => by unfold rec'; rfl
+  | .var x => by unfold rec'; rfl
+  | .op o ai => by unfold rec'; exact congrArg (op o ai) (rec_1_eq_rec_1'_ ai)
+
+private theorem rec_1_eq_rec_1'_ : ∀ ai, @rec_1 S O motive₁ motive₂ @bvar @var @op @nil @cons si ai = @rec_1' S O motive₁ motive₂ @bvar @var @op @nil @cons si ai
+  | .nil => by unfold rec_1'; rfl
+  | .cons a ai => by unfold rec_1'; exact congr (congrArg (cons a ai) (rec_eq_rec'_ a)) (rec_1_eq_rec_1'_ ai)
+
+end
+
+end rec
+
+@[csimp]
+private theorem rec_eq_rec' : @rec = @rec' := by
+  funext S O motive₁ motive₂ bvar var op nil cons s a
+  apply rec_eq_rec'_
+
+@[csimp]
+private theorem rec_1_eq_rec_1' : @rec_1 = @rec_1' := by
+  funext S O motive₁ motive₂ bvar var op nil cons si ai
+  apply rec_1_eq_rec_1'_
+
+def ndrec
+  {motive : S → Type u}
+  (bvar : ∀ s, Nat → motive s)
+  (var : ∀ {s}, Var s → motive s)
+  (op : ∀ {si s}, O si s → DList (Abt₁ O ·.2) si → DList (motive ·.2) si → motive s)
+: ∀ {a}, Abt₁ O a → motive a :=
+  @rec S O (λ s _ => motive s) (λ si _ => DList (motive ·.2) si) bvar var op DList.nil λ _ _ => DList.cons (α := _ × S) (β := (motive ·.2))
+
+end Abt₁
+
+variable {S : Type} (O : ∀ ⦃n⦄, (Fin n → List S × S) → S → Type) in
+inductive Abt₂ : S → Type
+  | bvar s (n : Nat) : Abt₂ s
+  | var (x : Var s) : Abt₂ s
+  | op {si : Fin n → _} (o : O si s) (ai : ∀ i, Abt₂ (si i).2) : Abt₂ s
+
+variable {S : Type} (O : ∀ ⦃n⦄, (Fin n → ((m : Nat) × (Fin m → S)) × S) → S → Type) in
+inductive Abt₃ : S → Type
+  | bvar s (n : Nat) : Abt₃ s
+  | var (x : Var s) : Abt₃ s
+  | op {si : Fin n → _} (o : O si s) (ai : ∀ i, Abt₃ (si i).2) : Abt₃ s
+
+variable [DecidableEq S] (s : S) in
+def bindCount : List S → Nat
+  | [] => 0
+  | t :: ts => bindCount ts + if t = s then 1 else 0
+
+variable {S : Type u} [DecidableEq S] (s : S) in
+def bindCount' : ((m : Nat) × (Fin m → S)) → Nat
+  | ⟨0, _⟩ => 0
+  | ⟨m + 1, ts⟩ => bindCount' ⟨m, ts ∘ .succ⟩ + if ts .zero = s then 1 else 0
+
+variable [DecidableEq S] {s : S} (x : Var s) in
+def Abt₁.bind : @Abt₁ S O t → Nat → Abt₁ O t :=
+  ndrec (motive := λ t => Nat → Abt₁ O t)
+    (λ t m _n => bvar t m)
+    (λ {t} y n => if h : t = s then if h ▸ y = x then bvar t n else var y else var y)
+    (λ o _ai ai' n => op o (ai'.map λ {b} f => f (n + bindCount s b.1)))
+
+variable [DecidableEq S] {s : S} (x : Var s) in
+def Abt₂.bind (n : Nat) : @Abt₂ S O t → Abt₂ O t
+  | bvar t m => bvar t m
+  | var y => if h : t = s then if h ▸ y = x then bvar t n else var y else var y
+  | op (si := si) o ai => op o λ i => bind (n + bindCount s (si i).1) (ai i)
+
+variable [DecidableEq S] {s : S} (x : Var s) in
+def Abt₃.bind (n : Nat) : @Abt₃ S O t → Abt₃ O t
+  | bvar t m => bvar t m
+  | var y => if h : t = s then if h ▸ y = x then bvar t n else var y else var y
+  | op (si := si) o ai => op o λ i => bind (n + bindCount' s (si i).1) (ai i)
+
+def Abt₁.op' [DecidableEq S] {s : S} (o : O si s) (ai : DList (λ b => DList Var b.1 × Abt₁ O b.2) si) : Abt₁ O s :=
+  .op o <| ai.map λ a => a.1.foldr (λ {t} x (a, n) => (bind x a (n t), λ u => if u = t then n u + 1 else n u)) (a.2, λ _ : S => 0) |>.1
+
+def Abt₂.op' [DecidableEq S] {s : S} (o : O si s) (ai : ∀ i, DList Var (si i).1 × Abt₂ O (si i).2) : Abt₂ O s :=
+  .op o λ i => (ai i).1.foldr (λ {t} x (a, n) => (bind x (n t) a, λ u => if u = t then n u + 1 else n u)) ((ai i).2, λ _ : S => 0) |>.1
+
+def Abt₃.op' [DecidableEq S] {s : S} (o : O si s) (ai : ∀ i, (∀ j, Var ((si i).1.2 j)) × Abt₃ O (si i).2) : Abt₃ O s :=
+  .op o λ i => FinTuple.foldr (λ {j} x (a, n) => (bind x (n ((si i).1.2 j)) a, λ u => if u = (si i).1.2 j then n u + 1 else n u)) ((ai i).2, λ _ : S => 0) (ai i).1 |>.1
+
+inductive O₁ : List (List Unit × Unit) → Unit → Type
+  | foo : O₁ [([], ()), ([], ())] ()
+  | bar : O₁ [([(), ()], ())] ()
+
+instance : ToString (O₁ si s) where
+  toString
+    | .foo => "foo"
+    | .bar => "bar"
+
+open FinTuple in
+inductive O₂ : ∀ ⦃n⦄, (Fin n → List Unit × Unit) → Unit → Type
+  | foo : O₂ ⟦([], ()), ([], ())⟧ ()
+  | bar : O₂ ⟦([(), ()], ())⟧ ()
+
+instance : ToString (O₂ si s) where
+  toString
+    | .foo => "foo"
+    | .bar => "bar"
+
+open FinTuple in
+inductive O₃ : ∀ ⦃n⦄, (Fin n → ((m : Nat) × (Fin m → Unit)) × Unit) → Unit → Type
+  | foo : O₃ ⟦(⟨_, ⟦⟧⟩, ()), (⟨_, ⟦⟧⟩, ())⟧ ()
+  | bar : O₃ ⟦(⟨_, ⟦(), ()⟧⟩, ())⟧ ()
+
+instance : ToString (O₃ si s) where
+  toString
+    | .foo => "foo"
+    | .bar => "bar"
+
+open DList in
+#reduce (.op' .bar ⟦(⟦23, 24⟧, .op .foo ⟦.var 23, .var 24⟧)⟧ : Abt₁ O₁ ())
+open FinTuple DList in
+#check (.op' .bar ⟦(⟦23, 24⟧, .op .foo ⟦.var 23, .var 24⟧)⟧ : Abt₂ O₂ ())
+open FinTuple in
+#check (.op' .bar ⟦(⟦23, 24⟧, .op .foo ⟦.var 23, .var 24⟧)⟧ : Abt₃ O₃ ())
+
+/-
+def Abt.op' [DecidableEq S] (o : O si s) (ai : ∀ i, (∀ j, Var' ((si i).1.2 j)) × Abt S O (si i).2) : Abt S O s :=
+  .op o λ i => FinTuple.foldr' (λ k x => bind _ x k) (ai i).2 (ai i).1
+
+def Abt.free [DecidableEq S] (s' : S) (a : Abt S O s) : Var' s' :=
+  let n := fv a
+  let v := h a (mkArray n true)
+  Id.run do
+  for (i, b) in v.toList.enum do
+    if b then
+      return ⟨i⟩
+  return ⟨n⟩
+where
+  fv {s}
+  | .fvar (s := s'') _ => if s'' = s' then 1 else 0
+  | .var _ _ => 0
+  | .op _ ai => FinTuple.foldr Nat.add 0 λ i => fv (ai i)
+  h {s}
+  | .fvar (s := s'') x, v => if s'' = s' then v.setD x.x false else v
+  | .var _ _, v => v
+  | .op _ ai, v => FinTuple.foldr (λ (f : _ → _) a => f a) v λ i => h (ai i)
+
+def Abt.unbind [DecidableEq S] {s' : S} (x : Var' s') (d : Nat) : Abt S O s → Abt S O s
+  | .fvar y => .fvar y
+  | .var s (y : Nat) =>
+    if h : s = s'
+    then
+      match compare y d with
+      | .gt => .var s (y - 1)
+      | .eq => h ▸ .fvar x
+      | .lt => .var s y
+    else .var s y
+  | .op (si := si) o ai => .op o λ i => (ai i).unbind x (d + liftAmt s' (si i).1)
+
+def Abt.unop [DecidableEq S] (o : O si s) (ai : ∀ i, Abt S O (si i).2) i : (∀ j, Var' ((si i).1.2 j)) × Abt S O (si i).2 :=
+  FinTuple.dfoldl
+    (β := λ k => (S → Nat) × ((j : Fin k) → Var' ((si i).1.2 (j.cast (Nat.pred_le_pred k.isLt)))) × Abt S O (si i).2)
+    (λ {j} (d, f, a) _ => let b := (si i).1.2 j; let x := a.free b; let d' s := if s = b then d s - 1 else d s; (d', Fin.revCases x f, a.unbind x (d' b)))
+    ((liftAmt · (si i).1), λ k => nomatch k, ai i)
+    (si i).1.2
+    |>.2
+
+variable [DecidableEq S] [∀ {n} si s, DecidableEq (@O n si s)] (b : Abt S O s) (x : Var' s) in
+def Abt.subst : Abt S O s' → Abt S O s'
+  | var s' y => var s' y
+  | fvar (s := s') y => if h : s' = s then if x.x = y.x then h ▸ b else fvar y else fvar y
+  | op o ai => op o λ i => subst (ai i)
+
+variable {S : Type} {O : ∀ ⦃n⦄, (Fin n → ((m : Nat) × (Fin m → S)) × S) → S → Type} in
+instance [DecidableEq S] [∀ {n} si s, ToString (@O n si s)] : ToString (Abt S O s) where
+  toString a := h (λ _ => 0) a
+where
+  h {s} (d : S → Nat) : Abt S O s → String
+  | .fvar x => x.toString ++ "'"
+  | .var s (x : Nat) => Var.toString (d s - 1 - x)
+  | .op (si := si) o ai => toString o ++ h' λ i => h'' d (si i).1 ++ h (λ s' => d s' + Abt.liftAmt s' (si i).1) (ai i)
+  h' : ∀ {n}, (Fin n → String) → String
+  | 0, _ => ""
+  | _ + 1, ai => "(" ++ String.join (List.intersperse "; " (FinTuple.toList ai)) ++ ")"
+  h'' (d : S → Nat) : (m : Nat) × (Fin m → S) → String
+  | ⟨0, _⟩ => ""
+  | ⟨_ + 1, si⟩ => String.join (List.intersperse ", " (FinTuple.foldl (λ (bs, d) b => (Var.toString (d b) :: bs, λ s => d s + if b = s then 1 else 0)) ([], d) si).1.reverse) ++ ". "
+
+instance (priority := low) [ToString α] : Repr α where
+  reprPrec x _ := toString x
+
+namespace ExampleAbt
+
+inductive S
+  | Exp
+deriving DecidableEq
+
+inductive O : ∀ ⦃n⦄, (Fin n → ((m : Nat) × (Fin m → S)) × S) → S → Type
+  | num : Nat → O ⟦⟧ .Exp
+  | plus : O ⟦(⟦⟧', .Exp), (⟦⟧', .Exp)⟧ .Exp
+  | times : O ⟦(⟦⟧', .Exp), (⟦⟧', .Exp)⟧ .Exp
+  | let : O ⟦(⟦⟧', .Exp), (⟦.Exp⟧', .Exp)⟧ .Exp
+
+abbrev Abt := _root_.Abt S O
+
+instance : ToString (O si s) where
+  toString := h
+where h
+  | .num n => s!"num[{n}]"
+  | .plus => "plus"
+  | .times => "times"
+  | .let => "let"
+
+inductive Exp
+  | var : Var' S.Exp → Exp
+  | num : Nat → Exp
+  | plus : Abt .Exp → Abt .Exp → Exp
+  | times : Abt .Exp → Abt .Exp → Exp
+  | let : Abt .Exp → Var' S.Exp → Abt .Exp → Exp
+  deriving Repr
+
+def Exp.in : Exp → Abt .Exp
+  | .var x => .fvar x
+  | .num n => .op (.num n) ⟦⟧ 
+  | .plus a b => .op .plus ⟦a, b⟧
+  | .times a b => .op .times ⟦a, b⟧
+  | .let a x b => .op' .let ⟦(⟦⟧, a), (⟦x⟧, b)⟧
+
+def Exp.out : Abt .Exp → Exp
+  | .fvar x => .var x
+  | .var _ x => .var ⟨x⟩
+  | .op (.num n) _ => .num n 
+  | .op .plus ai => .plus (ai 0) (ai 1)
+  | .op .times ai => .times (ai 0) (ai 1)
+  | .op .let ai => let ai' := Abt.unop .let ai; .let (ai' 0).2 ((ai' 1).1 .zero) (ai' 1).2
+
+def Exp'.var := (Exp.in <| Exp.var ·)
+def Exp'.num := (Exp.in <| Exp.num ·)
+def Exp'.plus := (Exp.in <| Exp.plus · ·)
+def Exp'.times := (Exp.in <| Exp.times · ·)
+def Exp'.let := (Exp.in <| Exp.let · · ·)
+
+theorem Exp.in_out : ∀ e, Exp.in (Exp.out e) = e
+  | .fvar x => rfl
+  | .var _ x => sorry
+  | .op (.num n) _ => congrArg (Abt.op _) <| funext λ i => nomatch i
+  | .op .plus ai => congrArg (Abt.op _) <| funext λ | 0 => rfl | 1 => rfl
+  | .op .times ai => congrArg (Abt.op _) <| funext λ | 0 => rfl | 1 => rfl
+  | .op .let ai => congrArg (Abt.op _) <| funext λ | 0 => rfl | 1 => sorry
+
+end ExampleAbt
+
+section
+open ExampleAbt Exp'
+#eval Exp'.let (plus (num 2) (num 3)) "z" (times (var "z") (num 5))
+#eval match Exp'.let (plus (num 2) (num 3)) "z" (times (var "z") (num 5)) with | .op .let ai => Abt.unop O.let ai | _ => unreachable!
+end
+
+inductive O : ∀ ⦃n⦄, (Fin n → ((m : Nat) × (Fin m → Unit)) × Unit) → Unit → Type
+  | zero : O ⟦(⟦⟧', ()), (⟦⟧', ())⟧ ()
+  | one : O ⟦(⟦()⟧', ())⟧ ()
+  | two : O ⟦(⟦(), ()⟧', ())⟧ ()
+
+instance : ToString (O si s) where
+  toString
+    | .zero => "zero"
+    | .one => "one"
+    | .two => "two"
+
+#eval Abt.op' O.one ⟦(⟦"x"⟧, .fvar "x")⟧
+#eval Abt.op' O.one ⟦(⟦"x"⟧, .fvar "y")⟧
+#eval Abt.op' O.two ⟦(⟦"x", "y"⟧, .fvar "x")⟧
+#eval Abt.op' O.two ⟦(⟦"x", "y"⟧, .fvar "y")⟧
+#eval Abt.op' O.two ⟦(⟦"x", "y"⟧, .fvar "z")⟧
+#eval Abt.op' O.two ⟦(⟦"x", "y"⟧, .op' .zero ⟦(⟦⟧, .fvar "x"), (⟦⟧, .fvar "y")⟧)⟧
+
+#eval match Abt.op' O.two ⟦(⟦"x", "y"⟧, .fvar "x")⟧ with | .op .two ai => Abt.unop O.two ai | _ => unreachable!
+#eval match Abt.op' O.two ⟦(⟦"x", "y"⟧, .fvar "y")⟧ with | .op .two ai => Abt.unop O.two ai | _ => unreachable!
+#eval match Abt.op' O.two ⟦(⟦"x", "y"⟧, .fvar "z")⟧ with | .op .two ai => Abt.unop O.two ai | _ => unreachable!
+#eval match Abt.op' O.two ⟦(⟦"x", "y"⟧, .op' .zero ⟦(⟦⟧, .fvar "y"), (⟦⟧, .fvar "x")⟧)⟧ with | .op .two ai => Abt.unop O.two ai | _ => unreachable!
+
+#eval Abt.op' O.one ⟦(⟦"x"⟧, .op' .one ⟦(⟦"y"⟧, .op .zero ⟦.fvar "x", .fvar "y"⟧)⟧)⟧
+#eval match Abt.op' O.one ⟦(⟦"x"⟧, .op' .one ⟦(⟦"y"⟧, .op .zero ⟦.fvar "x", .fvar "y"⟧)⟧)⟧ with | .op .one ai => Abt.unop O.one ai | _ => unreachable!
+#eval match Abt.op' O.one ⟦(⟦"x"⟧, .op' .one ⟦(⟦"y"⟧, .op .zero ⟦.fvar "x", .fvar "y"⟧)⟧)⟧ with | .op .one ai => (match Abt.unop O.one ai 0 |>.2 with | .op .one ai => Abt.unop O.one ai | _ => unreachable!) | _ => unreachable!
+
+/-
+variable (S : Type) (O : ∀ ⦃n⦄, (Fin n → (S → Nat) × S) → S → Type) in
+inductive CAbt : (S → Nat) → S → Type
+  | var s (x : Fin (X s)) : CAbt X s
+  | op (o : O si s) (ai : ∀ i, CAbt (λ s => X s + (si i).1 s) (si i).2) : CAbt X s
+
+def ClAbt S O := CAbt S O λ _ => 0
+-/
+
+/-
+def Nat.le.rec' {n} {motive : (a : Nat) → n.le a → Sort u}
+  (refl : motive n .refl)
+  (step : ∀ {m} a, motive m a → motive m.succ a.step) {a} t
+: motive a t := by
+  cases h : a - n
+    <;> have := Nat.sub_add_cancel t |>.symm |>.trans <| congrArg (· + n) h
+    <;> simp [this, Nat.succ_add]
+  . exact refl
+  . exact step (Nat.le_add_left n _) (rec' refl step _)
+  -/
+-/
