Bug.lean
@@ -1,0 +1,49 @@
+import Lean
+
+/-
+syntax "level% " level : term
+macro_rules
+  | `(level% ($l)) => `(level% $l)
+  | `(level% $i:ident) => `(Lean.Level.param $(Lean.quote i.getId))
+  | `(level% $n:num) => `(Lean.Level.ofNat $n)
+  | `(level% $l + $n) => `(Lean.Level.addOffset (level% $l) $n)
+  | `(level% imax $l $l') => `(Lean.Level.imax (level% $l) (level% $l'))
+-/
+
+partial def elabLevel : Lean.TSyntax `level → Lean.CoreM Lean.Level
+  | `(level| ($l)) => elabLevel l
+  | `(level| $i:ident) => return .param i.getId
+  | `(level| $n:num) => return .ofNat n.getNat
+  | `(level| $l + $n) => return .addOffset (← elabLevel l) n.getNat
+  | `(level| imax $l $l') => return .imax (←elabLevel l) (← elabLevel l')
+  | _ => Lean.Elab.throwUnsupportedSyntax
+
+partial def elabExpr : Lean.TSyntax `term → Lean.CoreM Lean.Expr
+  | `(($t)) => elabExpr t
+  | `($i:ident) => return .const i.getId []
+  | `(@$i:ident) => return .const i.getId []
+  | `($i:ident.{$l,*}) => return .const i.getId (← l.getElems.toList.mapM elabLevel)
+  | `(@$i:ident.{$l,*}) => return .const i.getId (← l.getElems.toList.mapM elabLevel)
+  | `(Sort $l) => return .sort (← elabLevel l)
+  | `(Type $l) => return .sort (.succ (← elabLevel l))
+  | `($t $ts*) => return Lean.mkAppN (← elabExpr t) (← ts.mapM elabExpr)
+  | _ => Lean.Elab.throwUnsupportedSyntax
+
+syntax "rdef " ident (".{" ident,+ "}")? " : " term " := " term : command
+
+open Lean Elab Command in
+elab_rules : command | `(rdef $name $[.{ $levelParams?,* }]? : $type := $value) => do
+  let levelParams :=
+    if let some levelParams := levelParams?
+    then levelParams.getElems.toList.map (·.getId)
+    else []
+  liftCoreM <| addDecl <| .defnDecl {
+    name := name.getId
+    levelParams
+    type := ← liftCoreM <| elabExpr type
+    value := ← liftCoreM <| elabExpr value
+    hints := .abbrev
+    safety := .safe
+  }
+
+rdef bug.{u} : @Eq.{imax 1 u + 2} (Type (imax 1 u)) (Sort (imax 1 u)) (Type (imax 1 u)) := @rfl.{imax 1 u + 2} (Type (imax 1 u)) (Sort (imax 1 u))
