Cubical.lean
@@ -1,0 +1,38 @@
+def I : Type := Squash Bool
+def i0 : I := .mk false
+def i1 : I := .mk true
+
+protected def I.lift₁ (f : Bool → Bool) : I → I :=
+  Quot.lift (λ x => .mk (f x)) λ _ _ h => Quot.sound h
+
+protected def I.lift₂ (f : Bool → Bool → Bool) : I → I → I :=
+  Quot.lift (λ x => Quot.lift (λ y => .mk (f x y)) λ _ _ h => Quot.sound h) λ x x' h => by
+    suffices (λ y => Squash.mk (f x y)) = (λ y => .mk (f x' y)) by
+      dsimp
+      funext _
+      congr
+    exact funext λ _ => Quot.sound h
+
+def I.and : I → I → I := I.lift₂ _root_.and
+def I.or : I → I → I := I.lift₂ _root_.or
+def I.not : I → I := I.lift₁ _root_.not
+
+def Path (x y : α) := { f : I → α // f i0 = x ∧ f i1 = y }
+
+instance {x y : α} : CoeFun (Path x y) (λ _ => I → α) where
+  coe p := p.1
+
+def Path.h0 (p : Path x y) : p i0 = x := p.2.1
+def Path.h1 (p : Path x y) : p i1 = y := p.2.2
+
+def refl (x : α) : Path x x :=
+  ⟨λ _ => x, rfl, rfl⟩
+
+example (p : Path x y) : Eq x y :=
+  p.h0.symm.trans ((congrArg p (Quot.sound trivial)).trans p.h1)
+
+def sym (p : Path x y) : Path y x :=
+  ⟨λ i => p (I.not i), p.h1, p.h0⟩
+
+def funExt {β : α → _} {f g : (x : α) → β x} (p : (x : α) → Path (f x) (g x)) : Path f g :=
+  ⟨λ i x => p x i, funext λ x => (p x).h0, funext λ x => (p x).h1⟩
