Option.lean
@@ -1,0 +1,39 @@
+instance : LawfulFunctor Option where
+  map_const := rfl
+  id_map
+    | none => rfl
+    | some _ => rfl
+  comp_map _ _
+    | none => rfl
+    | some _ => rfl
+
+instance : LawfulApplicative Option where
+  seqLeft_eq
+    | none, _ => rfl
+    | some _, none => rfl
+    | some _, some _ => rfl
+  seqRight_eq
+    | none, _ => rfl
+    | some _, none => rfl
+    | some _, some _ => rfl
+  pure_seq _ _ := rfl
+  map_pure _ _ := rfl
+  seq_pure
+    | none, _ => rfl
+    | some _, _ => rfl
+  seq_assoc
+    | _, _, none => rfl
+    | _, none, some _ => rfl
+    | none, some _, some _ => rfl
+    | some _, some _, some _ => rfl
+
+instance : LawfulMonad Option where
+  bind_pure_comp _
+    | none => rfl
+    | some _ => rfl
+  bind_map _ _ := rfl
+  pure_bind _ _ := rfl
+  bind_assoc
+    | none, _, _ => rfl
+    | some _, _, _ => rfl
+
