Search.lean
@@ -1,0 +1,39 @@
+@[simp]
+theorem Subarray.size_popFront (a : Subarray α) : a.popFront.size = a.size.pred := by
+  cases h : a.size with
+  | zero =>
+    have : ¬a.start < a.stop := by
+      rw [Nat.not_lt_eq, ← Nat.zero_add a.start]
+      exact Nat.le_add_of_sub_le <| Nat.le_of_eq h
+    simp [popFront, this]
+    exact h
+  | succ =>
+    rw [← h]
+    have : a.start < a.stop := by
+      dsimp [size] at h
+      have := Nat.le_of_eq h
+      sorry
+    simp [popFront, this]
+    rfl
+
+variable [BEq α] (x : α) (a : Subarray α)
+
+def linsearch (a : Subarray α) : Option Nat :=
+  if _ : 0 < a.size
+  then
+    if a[0] == x
+    then some 0
+    else linsearch a.popFront
+  else none
+termination_by _ => a.size
+
+def ilinsearch : Option Nat := Id.run do
+  for h : i in [:a.size] do
+    if a[i]'h.2 == x then
+      return some i
+  return none
+
+theorem ilinsearch_eq_linsearch : linsearch x a = ilinsearch x q := by
+  unfold linsearch ilinsearch
+  dsimp [Id.run]
+  sorry
