cps.lean
@@ -1,0 +1,198 @@
+import Lean.Elab.Command
+import Lean
+
+open Lean
+
+partial def getApp : Term → Term × Array Term
+  | `($t $ts*) => let (hd, tl) := getApp t; (hd, tl ++ ts)
+  | `(($t)) => getApp t
+  | stx => (stx, #[])
+
+partial def cps' (i : Ident) (n : Nat) (a : Array Term → MacroM Term) (stx : Term) : MacroM ((Term → MacroM Term) × Term) :=
+  let (hd, tl) := getApp stx
+  if hd == i then
+    if tl.size < n
+    then throw <| .error stx "function not fully applied"
+    else do
+      let (bs₁, tl₁) ← tl[:n].foldlM (λ (binds, tl) x => do
+        let (bind, y) ← cps' i n a x
+        return (binds <=< bind, tl.push y)
+      ) (pure, .mkEmpty n)
+      let tl₁ ← a tl₁
+      let (bs₂, tl₂) ← tl[n:].foldlM (λ (binds, tl) x => do
+        let (bind, y) ← cps' i n a x
+        return (binds <=< bind, tl.push y)
+      ) (pure, .mkEmpty (tl.size - n))
+      let b ← withFreshMacroScope `(__do_lift)
+      return (bs₁ <=< (λ bd => `($tl₁ >>= λ $b => $bd)) <=< bs₂, ← `($b $tl₂*))
+  else if let `(← $e) := stx then do
+    let (be, e) ← cps' i n a e
+    let b ← withFreshMacroScope `(__do_lift)
+    return (be <=< (λ bd => `($e >>= λ $b => $bd)), b)
+  else if let `(if $c then $t else $e) := stx then do
+    let (bc, c) ← cps' i n a c
+    let (bt, t) ← cps' i n a t
+    let (be, e) ← cps' i n a e
+    let t ← bt <| ← `(pure $t)
+    let e ← be <| ← `(pure $e)
+    let b ← withFreshMacroScope `(__do_lift)
+    return (bc <=< λ bd => `((if $c then $t else $e) >>= λ $b => $bd), b)
+  else if let `(match $[$d],* with $[| $[$lhs,*]|* => $rhs]*) := stx then do
+    let (bd, d) ← d.foldlM (λ (bd, d) arg => do
+      let (bind, arg') ← cps' i n a ⟨arg.raw[1]⟩
+      return (bd <=< bind, d.push ⟨arg.raw.setArg 1 arg'⟩)
+    ) (pure, .mkEmpty d.size)
+    let rhs ← rhs.mapM λ rhs => do
+      let (brhs, rhs) ← cps' i n a rhs
+      brhs <| ← `(pure $rhs)
+    let b ← withFreshMacroScope `(__do_lift)
+    return (bd <=< λ bd => `((match $[$d],* with $[| $[$lhs,*]|* => $rhs]*) >>= λ $b => $bd), b)
+  else do
+    let (binds, args) ← stx.raw.getArgs.foldlM (λ (binds, args) arg => do
+      let (bind, arg) ← cps' i n a ⟨arg⟩
+      return (binds <=< bind, args.push arg.raw)
+    ) (pure, .mkEmpty stx.raw.getNumArgs)
+    return (binds, ⟨stx.raw.setArgs args⟩)
+
+def cps (i : Ident) (n : Nat) (a : Array Term → MacroM Term := λ a => `($i $a*)) (t : Term) : MacroM Term := do
+  let (b, t) ← cps' i n a t
+  b <| ← `(pure $t)
+
+/-
+macro "cps% " i:ident n:num t:term : term => (cps i n.getNat) t
+-/
+
+/-
+elab "#cps " i:ident n:num t:term : command => do
+  let t' ← Elab.liftMacroM <| (cps i n.getNat) t
+  logInfoAt t t'
+-/
+
+/-
+elab tk:"#expand " t:term : command => do
+  let t ← Elab.liftMacroM <| expandMacros t
+  logInfoAt tk t
+-/
+
+def Function.curry (f : α × β → δ) (x : α) (y : β) : δ := f (x, y)
+
+structure Fix (α : Sort u) (C : α → Type v) [I : WellFoundedRelation α] (m : Type v → Type w) [Monad m] where
+  fix : (∀ x, (∀ y, I.rel y x → m (C y)) → m (C x)) → ∀ x, C x
+
+open Lean.Parser in
+@[command_parser]
+def fdef := leading_parser
+  "fdef " >> ident >> " : " >> termParser >> Term.matchAlts
+
+macro_rules
+  | `(fdef $n : $t₁ → $t₂ $[| $[$l,*]|* => $r]*) => do
+    let ns := r.map λ _ => n
+    let rs ← r.mapM <| cps n 1 (λ a => `($n $a* (by decreasing_tactic)))
+    let m := mkIdent `m
+    let fix := mkIdent `fix
+    `(def $n [Monad $m] {$fix : Fix $t₁ (λ _ => $t₂) $m} : $t₁ → $t₂ := $(fix).fix λ
+      $[| $[$l,*]|* => λ $ns => $rs]*)
+
+macro_rules
+  | `(fdef $n : $t₁ → $t₂ → $t₃ $[| $[$l₁, $l₂]|* => $r]*) => do
+    let ns := r.map λ _ => n
+    let rs ← r.mapM <| cps n 2 (λ a => `($n ($(a[0]!), $(a[1:]),*) (by decreasing_tactic)))
+    let m := mkIdent `m
+    let fix := mkIdent `fix
+    `(def $n [Monad $m] {$fix : Fix ($t₁ × $t₂) (λ _ => $t₃) $m} : $t₁ → $t₂ → $t₃ := Function.curry <| $(fix).fix λ
+      $[| $[($l₁, $l₂)]|* => λ $ns => $rs]*)
+
+private def WellFounded.fix' {α : Sort u} {C : α → Sort v} {r} (hwf : WellFounded r) (F : ∀ x, (∀ y, r y x → C y) → C x) x : C x :=
+  F x λ y _ => fix' hwf F y
+termination_by' ⟨r, hwf⟩
+
+@[csimp]
+private theorem WellFounded.fix_eq_fix' : @fix = @fix' := by
+  funext _ _ _ _ _ _
+  unfold WellFounded.fix'
+  apply fix_eq
+
+def Fix.basic {α : Sort u} {C : α → Type v} [I : WellFoundedRelation α] : Fix α C Id where
+  fix := WellFounded.fix I.wf
+
+def Fix.memo {α : Type u} {β : Type (max u v)} [I : WellFoundedRelation α] [Ord α] : Fix α (λ _ => β) (StateM (Lean.RBMap α β compare)) where
+  fix f := StateT.run' (s := .empty) ∘ WellFounded.fix I.wf λ x ih m =>
+    match m.find? x with
+    | some y => (y, m)
+    | none =>
+      let (y, m) := f x ih m
+      (y, m.insert x y)
+
+def Fix.dbgTrace {α : Type u} {C : α → Type v} [WellFoundedRelation α] {m : Type v → Type w} [Monad m] (fix : Fix α C m) [ToString α] : Fix α C m where
+  fix f := fix.fix λ x => dbg_trace s!"f {x}"; f x
+
+fdef fib : Nat → Nat
+  | 0 => 0
+  | 1 => 1
+  | n + 2 => fib (n + 1) + fib n
+
+#eval fib (fix := .dbgTrace .basic) 6
+#eval fib (fix := .dbgTrace .memo) 6
+
+instance [Ord α] [Ord β] : Ord (α × β) where
+  compare x y :=
+    match compare x.1 y.1 with
+    | .eq => compare x.2 y.2
+    | o => o
+
+fdef ack : Nat → Nat → Nat
+  | 0, n => n + 1
+  | m + 1, 0 => ack m 1
+  | m + 1, n + 1 => ack m (ack (m + 1) n)
+
+#eval ack (fix := .dbgTrace .basic) 2 1
+#eval ack (fix := .dbgTrace .memo) 2 1
+
+def le (x y : Nat) : Bool :=
+  dbg_trace s!"{x} ≤ {y}"
+  x ≤ y
+
+def insert' : Nat → List Nat → List Nat
+  | x, [] => [x]
+  | x, y :: l =>
+    if le x y
+    then x :: y :: l
+    else y :: insert' x l
+
+fdef insert : Nat → List Nat → List Nat
+  | x, [] => [x]
+  | x, y :: l =>
+    if le x y
+    then x :: y :: l
+    else y :: insert x l
+
+#eval insert' 2 [1, 3, 4]
+#eval insert (fix := .dbgTrace .basic) 2 [1, 3, 4]
+
+open Lean.Parser in
+@[command_parser]
+def mdef := leading_parser
+  "mdef " >> ident >> " : " >> termParser >> Term.matchAlts
+
+macro_rules
+  | `(mdef $n : $t₁ → $t₂ $[| $[$l,*]|* => $r]*) => do
+    let rs ← r.mapM <| cps n 1
+    `(def $n : $t₁ → $t₂ := λ
+      $[| $[$l,*]|* => $rs]*)
+
+def mul (x y : Nat) : Nat :=
+  dbg_trace s!"{x} * {y}"
+  x * y
+
+mdef prod' : List Nat → Option Nat
+  | [] => 1
+  | x :: l =>
+    if x == 0
+    then ← none
+    else x |> mul <| prod' l
+
+def prod l := prod' l |>.getD 0
+
+#eval prod [1, 2, 3, 4, 5]
+#eval prod [0, 2, 3, 4, 5]
+#eval prod [1, 2, 3, 4, 0]
