sorting/Macro.lean
@@ -1,0 +1,82 @@
+import Lean
+
+#check do
+  let mut i := 1
+  for _ in Lean.Loop.mk with h : 0 < i := Nat.lt_succ_self 0 do
+    if i ≥ 10 then
+      break
+    else
+      IO.println i
+      i := i + 1
+      --have := by exact Nat.le_step h
+      continue
+  --have _ : 0 < i := h
+  IO.println i
+
+open Lean
+
+partial def getVars (stx : Syntax) : MacroM (List Ident) :=
+  let rec visit : Syntax → StateT (List Ident) MacroM Unit
+    | stx@(.ident _ _ _ _) => modify (⟨stx⟩ :: ·)
+    | .node _ _ args => args.forM visit
+    | _ => return ()
+  return (← visit stx []).2
+
+partial def replaceVar (before : Ident) (after : Syntax) : Syntax → Syntax
+  | stx@(.ident _ _ _ _) => if stx == before then after else stx
+  | .node info kind args => .node info kind <| args.map <| replaceVar before after
+  | stx => stx
+
+def getDoSeqElems (doSeq : Syntax) : Array Syntax :=
+  if doSeq.getKind == ``Parser.Term.doSeqBracketed then
+    doSeq[1].getArgs.map (·[0])
+  else if doSeq.getKind == ``Parser.Term.doSeqIndent then
+    doSeq[0].getArgs.map (·[0])
+  else
+    #[]
+
+def mkDoSeq' (doElems : Array (MacroM Syntax)) : MacroM Syntax :=
+  return Lean.Elab.Term.Do.mkDoSeq (← doElems.mapM id)
+
+partial def insertBeforeContinue (el : Syntax) : Syntax → MacroM Syntax
+  | stx@(.node info kind args) =>
+    if kind == ``Lean.Parser.Term.doContinue
+    then `(doElem| do $(⟨Lean.Elab.Term.Do.mkDoSeq #[el, stx]⟩))
+    else return .node info kind (← args.mapM (insertBeforeContinue el))
+  | stx => return stx
+
+syntax "for " Parser.Term.doForDecl,+ "with " ident " : " term " := " term "; do " doSeq : doElem
+macro_rules | `(doElem| for $i in $e with $h : $t := $v; do $s) => do
+  let [x] := ← getVars t
+    | Macro.throwUnsupported
+  let s := getDoSeqElems (replaceVar x (← `(x)) s)
+  let t' := replaceVar x (← `(x)) t
+
+  let s ← s.mapM <| insertBeforeContinue <| ← `(doElem| h := ⟨x, by assumption⟩)
+
+  let s := s.insertAt 0 <| ← `(doElem| let $h : $(⟨t'⟩) := h.2)
+  let s := s.insertAt 0 <| ← `(doElem| let mut x := h.1)
+
+  let s : TSyntax `Lean.Parser.Term.doSeq := ⟨Lean.Elab.Term.Do.mkDoSeq s⟩
+
+  let seq := ⟨← mkDoSeq' #[
+    `(doElem| let mut h : { $x // $t } := ⟨$x, $v⟩),
+    `(doElem| for $i in $e do $s),
+    --`(doElem| $x := h.1)
+    return .node1 .none ``Lean.Parser.Term.doReassign <| .node5 .none ``Lean.Parser.Term.letIdDecl x mkNullNode mkNullNode mkNullNode (← `(h.1)),
+    `(doElem| let $h : $t := h.2)
+  ]⟩
+  `(doElem| do $seq)
+
+#check do
+  let mut i := 1
+  for _ in Lean.Loop.mk with h : 0 < i := Nat.lt_succ_self 0; do
+    if i ≥ 10 then
+      break
+    else
+      IO.println i
+      i := i + 1
+      have := by exact Nat.le_step h
+      continue
+  have _ : 0 < i := h
+  IO.println i
