sorting/Sorting.lean
@@ -1,0 +1,542 @@
+import Lean
+import Sorting.List
+import Sorting.Tactic
+
+class ComparisonSort (f : ∀ {m} [Monad m] {α}, (α → α → m Bool) → List α → m (List α)) where
+  perm (le : α → α → Bool) l : List.Perm (f (m := Id) le l) l
+  sort (le : α → α → Bool) (hle : ∀ {x y}, ¬le x y → le y x) l : List.Chain (le · ·) (f (m := Id) le l)
+
+section
+
+variable {m} [Monad m] {α} (le : α → α → m Bool)
+
+def insert (x : α) : List α → m (List α)
+  | [] => return [x]
+  | y :: l => do
+    if ← le x y
+    then return x :: y :: l
+    else return y :: (← insert x l)
+
+def insertionSort : List α → m (List α)
+  | [] => return []
+  | x :: l => do insert le x (← insertionSort l)
+
+end
+
+instance : ComparisonSort @insertionSort where
+  perm le l := by
+    induction l <;> simp [insertionSort]
+    case cons l ih =>
+      apply .trans _ (.cons _ ih)
+      clear ih
+      generalize insertionSort (m := Id) le l = l
+      induction l <;> simp [insert]
+      split <;> simp [*]
+
+  sort le hle l := by
+    induction l <;> simp [insertionSort]
+    case cons l ih =>
+      generalize insertionSort (m := Id) le l = l at ih
+      induction l <;> simp [insert]
+      case cons ih' =>
+        split with h
+        . simp [h, ih]
+        . cases ih <;> simp [insert, hle h] at ih' ⊢
+          case cons h₁ h₂ =>
+            specialize ih' h₁
+            split with h' <;> simp [h'] at ih' <;> simp [hle h, h₂, h', ih']
+
+section
+
+variable [Monad m] {α} (le : α → α → m Bool)
+
+def select (x : α) : List α → m (α × List α)
+  | [] => return (x, [])
+  | y :: l => do
+    if ← le x y
+    then do
+      let s ← select x l
+      return (s.1, y :: s.2)
+    else do
+      let s ← select y l
+      return (s.1, x :: s.2)
+
+def selectionSort' : Nat → List α → m (List α)
+  | 0, _ => return []
+  | _, [] => return []
+  | n + 1, x :: l => do
+    let s ← select le x l
+    return s.1 :: (← selectionSort' n s.2)
+
+def selectionSort (l : List α) : m (List α) :=
+  selectionSort' le l.length l
+
+end
+
+theorem perm_select x l : List.Perm (let s := select (m := Id) le x l; s.1 :: s.2) (x :: l) := by
+  induction l generalizing x <;> simp [select]
+  split <;> simp [*]
+
+structure TotalPreorder (r : α → α → Prop) where
+  trans : r x y → r y z → r x z
+  total x y : r x y ∨ r y x
+  refl x : r x x := (total x x).elim id id
+  ofNot : ¬r x y → r y x := (total y x).elim id ∘ (False.elim ∘ ·)
+
+theorem sort_select (le : α → α → Bool) (hle : TotalPreorder (le · ·)) x l : let s := select (m := Id) le x l; ∀ y, List.Mem y s.2 → le s.1 y := by
+  induction l generalizing x <;> simp [select, List.foldr]
+  case nil =>
+    intro _ h
+    cases h
+  case cons y l ih =>
+    split with h'
+    . specialize ih x
+      intro
+      | _, .tail _ h => exact ih _ h
+      | _, .head _ =>
+        have := (perm_select (le := le) x l).symm.mem (.head _)
+        simp at this ⊢
+        generalize hz : (select (m := Id) le x l).fst = z at this
+        cases this
+        . exact h'
+        . cases hz
+          apply hle.trans (ih _ _) h'
+          assumption
+    . specialize ih y
+      intro
+      | _, .tail _ h => exact ih _ h
+      | _, .head _ =>
+        have := (perm_select (le := le) y l).symm.mem (.head _)
+        simp at this
+        generalize hz : (select (m := Id) le y l).fst = z at this
+        cases this
+        . exact hle.ofNot h'
+        . cases hz
+          apply hle.trans (ih _ _) (hle.ofNot h')
+          assumption
+
+theorem perm_selectionSort (le : α → α → Bool) l : List.Perm (selectionSort (m := Id) le l) l := by
+  unfold selectionSort
+  generalize hn : l.length = n
+  induction n generalizing l <;> cases l <;> cases hn <;> simp [selectionSort']
+  case succ ih =>
+    exact .trans (.cons _ (ih _ (Nat.succ.inj (perm_select _ _).length))) (perm_select _ _)
+
+instance : ComparisonSort @selectionSort where
+  perm := perm_selectionSort
+
+  sort le hle l := by
+    unfold selectionSort
+    replace hle : TotalPreorder (le · ·) := sorry
+    generalize hn : l.length = n
+    induction n generalizing l <;> cases l <;> cases hn <;> simp [selectionSort']
+    case succ x l ih =>
+      specialize ih (select (m := Id) le x l).snd (Nat.succ.inj (perm_select _ _).length)
+      simp at ih
+      have := sort_select le hle x l
+      generalize hL : selectionSort' (m := Id) le (List.length l) (select (m := Id) le x l).2 = L at ih
+      cases L with
+      | nil => exact .singleton _
+      | cons y L =>
+        apply .cons (this _ _) ih
+        have : List.Mem y (y :: L) := List.Mem.head _
+        rw [← hL] at this
+        rw [← Nat.succ.inj (perm_select _ _).length] at this
+        exact (perm_selectionSort le (select (m := Id) le x l).snd).mem this
+
+def isort [Monad m] (le : α → α → m Bool) : List α → m (List α)
+  | [] => return []
+  | l@(h :: _) => have := Inhabited.mk h; do
+    let mut l := Array.mk l
+    let mut i := l.size - 1
+    while i > 0 do
+      let x := l[i - 1]!
+      let mut j := i
+      while j < l.size do
+        if ← le x l[j]! then break
+        l := l.set! (j - 1) l[j]!
+        j := j + 1
+      l := l.set! (j - 1) x
+      i := i - 1
+    return l.data
+
+def logLE (x y : Nat) : IO Bool := do
+  IO.println s!"{x} ≤ {y}"
+  return x ≤ y
+
+#eval insertionSort logLE [1, 2, 3, 4]
+#eval insertionSort logLE [4, 3, 2, 1]
+
+#eval isort logLE [1, 2, 3, 4]
+#eval isort logLE [4, 3, 2, 1]
+
+class SetElem (cont idx) (elem dom : outParam _) extends GetElem cont idx elem dom where
+  setElem (xs : cont) (i : idx) (h : dom xs i) : elem → cont
+
+export SetElem (setElem)
+
+def setElem! [SetElem cont idx elem dom] [Inhabited cont] (xs : cont) (i : idx) [Decidable (dom xs i)] : elem → cont :=
+  if h : _ then setElem xs i h else panic! "index out of bounds"
+
+macro "(" x:term " with " "[" i:term "]" " := " v:term ")" : term =>
+  `(setElem $x $i (by get_elem_tactic) $v)
+
+macro "(" x:term " with " "[" i:term "]'" h:term " := " v:term ")" : term =>
+  `(setElem $x $i $h $v)
+
+macro "(" x:term " with " "[" i:term "]" noWs "!" " := " v:term ")" : term =>
+  `(setElem! $x $i $v)
+
+instance : SetElem (Array α) Nat α λ a i => i < a.size where
+  setElem xs i h := xs.set ⟨i, h⟩
+
+def FixedArray α n := { a : Array α // a.size = n }
+
+namespace FixedArray
+
+def idx {a : FixedArray α n} (i : Fin n) : Fin a.1.size :=
+  ⟨i.1, by rw [a.2]; exact i.2⟩
+
+def get (a : FixedArray α n) (i : Fin n) : α :=
+  a.1.get (idx i)
+
+def set (a : FixedArray α n) (i : Fin n) (v : α) : FixedArray α n :=
+  ⟨a.1.set (idx i) v, (Array.size_set _ _ _).trans a.2⟩
+
+instance : GetElem (FixedArray α n) (Fin n) α λ _ _ => True where
+  getElem a i _ := a.get i
+
+instance : GetElem (FixedArray α n) Nat α λ _ i => i < n where
+  getElem a i h := a.get ⟨i, h⟩
+
+instance [Inhabited α] : Inhabited (FixedArray α n) where
+  default := ⟨⟨.replicate n default⟩, List.length_replicate n _⟩
+
+instance : SetElem (FixedArray α n) (Fin n) α λ _ _ => True where
+  setElem a i _ := a.set i
+
+instance : SetElem (FixedArray α n) Nat α λ _ i => i < n where
+  setElem a i h := a.set ⟨i, h⟩
+
+end FixedArray
+
+def runList (f : ∀ n, StateM (FixedArray α n) Unit) (a : List α) : List α :=
+  (f a.length ⟨⟨a⟩, rfl⟩).2.1.1
+
+namespace Magic
+
+open Lean
+
+scoped macro (name := m₁) "ℓ" noWs "[" i:term "]" : term => `((← get)[$i])
+scoped macro (name := m₂) "ℓ" noWs "[" i:term "]" noWs "!" : term => `((← get)[$i]!)
+scoped macro (name := m₃) "ℓ" noWs "[" i:term "]'" h:term : term => `((← get)[$i]'$h)
+
+scoped macro "ℓ" noWs "[" i:term "]" " := " v:term : term => `(modify λ xs => (xs with [$i] := $v))
+scoped macro "ℓ" noWs "[" i:term "]" noWs "!" " := " v:term : term => `(modify λ xs => (xs with [$i]! := $v))
+scoped macro "ℓ" noWs "[" i:term "]'" h:term " := " v:term : term => `(modify λ xs => (xs with [$i]'$h := $v))
+
+def doMacros : NameSet := .ofList [``m₁, ``m₂, ``m₃]
+
+partial def expandDoMacros (stx : Syntax) : MacroM Syntax :=
+  match stx with
+  | .node info kind args => do
+    if doMacros.contains kind then
+      if let some stx := ← expandMacro? stx then
+        return ← expandDoMacros stx
+    return .node info kind (← args.mapM expandDoMacros)
+  | _ => return stx
+
+scoped macro (name := processedDoMacros) "processedDoMacros% " t:term : term => return t
+
+def processDoMacros (stx : TSyntax `term) : MacroM (TSyntax `term) :=
+  if stx.raw.getKind == ``processedDoMacros
+  then throw .unsupportedSyntax
+  else do `(processedDoMacros% $(⟨← expandDoMacros stx⟩))
+
+scoped macro_rules | `(doElem| return $t) => do `(doElem| return $(← processDoMacros t))
+-- scoped macro_rules | `(doElem| $t:term) => do `(doElem| $(← processDoMacros t))
+scoped macro_rules | `(doElem| $t:term) => return .node1 (← MonadRef.mkInfoFromRefPos) `Lean.Parser.Term.doExpr (← processDoMacros t)
+scoped macro_rules | `(doElem| let $i := $t) => do `(doElem| let $i := $(← processDoMacros t))
+scoped macro_rules | `(doElem| if $[$h :]? $c then $t $[else $e]?) => do `(doElem| if $[$h :]? $(← processDoMacros c) then $t $[else $e]?)
+
+end Magic
+
+theorem Nat.succ_pred' (h : 0 < n) : n - 1 + 1 = n :=
+  succ_pred (ne_of_lt h).symm
+
+theorem Nat.lt_trans' {n m k : Nat} (h₁ : n ≤ m) (h₂ : m < k) : n < k :=
+  Nat.le_trans (succ_le_succ h₁) h₂
+
+theorem Nat.pred_lt_of_lt (h : m < n) : m - 1 < n := lt_trans' (pred_le m) h
+theorem Nat.pred_lt_of_le (h' : 0 < m) (h : m ≤ n) : m - 1 < n := Nat.le_trans (Nat.le_of_eq (succ_pred' h')) h
+
+macro_rules | `(tactic| get_elem_tactic_trivial) => `(tactic| apply Nat.pred_lt_of_lt; get_elem_tactic_trivial)
+
+open Magic in
+def isort' : List Nat → List Nat := runList λ n => do
+  let mut i := n - 1
+  while 0 < i do
+    let x := ℓ[i - 1]!
+    let mut j := i
+    while h : j < n do
+      if x ≤ ℓ[j] then break else
+        ℓ[j - 1] := ℓ[j]
+        j := j + 1
+    ℓ[j - 1]! := x
+    i := i - 1
+
+open Magic in
+def isort'' : List Nat → List Nat := runList λ n => do
+  let mut i : { i // 0 < i → i - 1 < n } := ⟨n - 1, λ h => Nat.le_trans (Nat.pred_lt' h) (Nat.pred_le n)⟩
+  while h : 0 < i.1 do
+    let x := ℓ[i.1 - 1]'(i.2 h)
+    let mut j : { j // 0 < j ∧ j ≤ n } := ⟨i.1, h, Nat.succ_pred' h ▸ i.2 h⟩
+    while h : j < n do
+      if x ≤ ℓ[j.1] then break else
+        ℓ[j.1 - 1] := ℓ[j.1]
+        j := ⟨j.1 + 1, Nat.lt.step j.2.1, h⟩
+    ℓ[j.1 - 1]'(Nat.pred_lt_of_le j.2.1 j.2.2) := x
+    i := ⟨i.1 - 1, λ h => Nat.le_trans (Nat.succ_le_succ (Nat.pred_le (i.1 - 1))) (i.2 (Nat.le_trans h (Nat.pred_le i.1)))⟩
+
+def isortv (l : Array Nat) : Array Nat := Id.run do
+  let mut l := l
+  let mut i := l.size - 1
+  while i > 0 do
+    let x := l[i - 1]!
+    let mut j := i
+    while j < l.size do
+      if x ≤ l[j]! then break
+      l := l.set! (j - 1) l[j]!
+      j := j + 1
+    l := l.set! (j - 1) x
+    i := i - 1
+  return l
+
+/-
+open Lean in
+partial def canPanic (name : Name) : CoreM (List Name) := do
+  let rec visit parent name : StateT (NameMap Name) CoreM Unit := do
+    if (← get).contains name then return
+    modify (·.insert name parent)
+    if let some value := (← getConstInfo name).value? then
+      value.getUsedConstants.forM (visit name)
+  let parents := (← visit name name .empty).2
+  let root := ← do
+    for name in [``panicCore, ``Array.get!, ``Array.set!] do
+      if parents.contains name then
+        return some name
+    return none
+  let mut some name := root
+    | return []
+  let mut names := []
+  repeat
+    let some parent := parents.find? name
+      | break
+    names := name :: names
+    if name == parent then break
+    name := parent
+  return names
+  -- change to namemap boolean, initially only known bad, and update to true each time
+
+#eval canPanic ``isort'
+-/
+
+/-
+open Lean in
+partial def getUsedConstants (name : Name) : CoreM (Array Name) := do
+  let rec visit name : StateT (NameSet × Array Name) CoreM Unit := do
+    if (← get).1.contains name then
+      return
+    modify fun (visited, names) => (visited.insert name, names)
+    let info ← getConstInfo name
+    info.type.getUsedConstants.forM visit
+    if let some value := info.value? then
+      value.getUsedConstants.forM visit
+    match ← getConstInfo name with
+    | .axiomInfo info => modify fun (visited, names) => (visited, names.push info.name)
+    | .opaqueInfo info => modify fun (visited, names) => (visited, names.push info.name)
+    | .quotInfo info => modify fun (visited, names) => (visited, names.push info.name)
+    | _ =>
+      if isExtern (← getEnv) name then
+        modify fun (visited, names) => (visited, names.push info.name)
+  return (← visit name (.empty, #[])).2.2
+
+deriving instance Repr for Lean.ExternEntry
+deriving instance Repr for Lean.ExternAttrData
+
+#eval getUsedConstants ``isort'
+-/
+
+/-
+#check Lean.isStructureLike
+deriving instance Repr for Lean.StructureInfo
+
+structure Foo where
+  a : Nat
+  b : Nat
+
+structure Bar extends Foo where
+  {c : Nat}
+  [d : Nat]
+
+structure Baz where
+  e : Bar
+  f : Nat := by simp
+
+section
+
+open Lean
+
+#eval show CoreM _ from do return getStructureInfo? (← getEnv) ``Foo
+#eval show CoreM _ from do return getStructureInfo? (← getEnv) ``Bar
+#eval show CoreM _ from do return getStructureInfo? (← getEnv) ``Baz
+
+end
+-/
+
+/-
+inductive Coroutine (Out In α : Type)
+  | return (x : α)
+  | yield (out : Out) (cont : In → Coroutine Out In α)
+
+def Coroutine.bind (f : α → Coroutine Out In β) : Coroutine Out In α → Coroutine Out In β
+  | .return x => f x
+  | .yield out cont => .yield out λ in' => bind f (cont in')
+
+instance : Monad (Coroutine Out In) where
+  pure := .return
+  bind x f := .bind f x
+
+def M.yield (out : Out) : Coroutine Out In In :=
+  .yield out .return
+
+partial def loop [Inhabited α] [Monad m] : m α := loop
+
+def runC [Inhabited α] [Monad m] (f : Out → m In) (co : Coroutine Out In α) : m α := do
+  let mut co := co
+  repeat
+    match co with
+    | .return x => return x
+    | .yield out cont => co := cont (← f out)
+  loop
+
+macro "yield " t:term : term => `(← M.yield $t)
+
+#check do _ := ← M.yield ()
+#check do _ := yield ()
+
+def foo : Coroutine Nat Nat Bool := do
+  let x := yield 100
+  return x > 5
+
+#eval runC (λ x => do IO.println x; return x) foo
+-/
+
+/-
+section
+
+variable [I : LE α] [DecidableRel I.le]
+
+def le [Monad m] (x y : α) : m Bool :=
+  return x ≤ y
+
+def timeLE (x y : α) : StateM Nat Bool :=
+  fun n => (x ≤ y, n + 1)
+
+def insertionSortTime (l : List α) : Nat :=
+  insertionSort timeLE l 0 |>.2
+
+end
+
+-- this holds for any soted list
+
+def List.rangeAux' (m : Nat) : Nat → List Nat
+  | 0 => []
+  | n + 1 => m :: rangeAux' (m + 1) n
+
+def List.range' : Nat → List Nat :=
+  List.rangeAux' 0
+
+theorem List.length_rangeAux' (m) : ∀ n, length (rangeAux' m n) = n
+  | 0 => rfl
+  | n + 1 => congrArg _ <| length_rangeAux' (m + 1) n
+
+theorem List.length_range' : ∀ n, length (range' n) = n :=
+  length_rangeAux' 0
+
+theorem insertM_range : insertM timeLE k (.rangeAux' (k + 1) (n + 1)) t = (.rangeAux' k (n + 2), t + 1) := by
+  simp [insertM, timeLE, k.le_succ]
+  rfl
+
+theorem insertionSortM_range : insertionSortM timeLE (.rangeAux' k (n + 1)) t = (.rangeAux' k (n + 1), t + n) := by
+  induction n generalizing k with
+  | zero => rfl
+  | succ n ih =>
+    unfold insertionSortM List.rangeAux'
+    simp [bind, StateT.bind, ih]
+    exact insertM_range
+
+example (n : Nat) : ∃ l : List Nat, l.length = n ∧ insertionSortTime l = n - 1 :=
+  .intro (.range' n) <| .intro (List.length_range' n) <| by
+    cases n with
+    | zero => rfl
+    | succ n => simp [insertionSortTime, List.range', insertionSortM_range, Nat.succ_sub_succ]
+
+theorem List.length_iota : ∀ n, length (iota n) = n
+  | 0 => rfl
+  | n + 1 => congrArg _ <| length_iota n
+
+theorem insertM_iota : insertM timeLE (k + 1) (.iota k) t = (.iota (k + 1), t + k) := by
+  sorry
+
+example (n : Nat)
+
+#eval List.range 5
+
+#eval insertionSortTime [1]
+#eval insertionSortTime [4, 3, 2, 1, 6]
+-/
+
+/-
+@[simp]
+def List.concatMap (f : α → List β) : List α → List β
+  | [] => []
+  | x :: l => f x ++ concatMap f l
+
+instance : Monad List where
+  pure x := [x]
+  bind l := l.concatMap
+
+def maxLE (_ _ : α) : StateT Nat List Bool :=
+  fun n => [(false, n + 1), (true, n + 1)]
+
+def insertionSortTime' (n : Nat) : Nat :=
+  insertionSort maxLE (.range n) 0 |>.foldl (fun x (_, y) => .max x y) 0
+
+def ContT (r : Type u) (m : Type u → Type v) (α : Type w) :=
+  (α → m r) → m r
+
+instance [Monad m] : Monad (ContT r m) where
+  pure x k := k x
+  bind f g k := f λ x => g x k
+
+abbrev Cont (r : Type u) (α : Type v) := ContT r Id α
+
+def maxLE' (_ _ : α) : Cont Nat Bool :=
+  λ k =>
+    let r : Nat := k false
+    let s : Nat := k true
+    max r s + 1
+
+def maxLE'' (_ _ : α) : Cont (Nat × List α) Bool :=
+  λ k =>
+    let r := k false
+    let s := k true
+    if r.1 ≤ s.1
+    then (s.1 + 1, s.2)
+    else (r.1 + 1, r.2)
+
+#eval insertionSort maxLE (.range 5) 0
+#eval insertionSort maxLE' (.range 5) λ _ => 0
+#eval insertionSort maxLE'' (.range 5) λ l => (0, l)
+-/
