sorting/Sorting/Range.lean
@@ -1,0 +1,52 @@
+structure Range where
+  start : Nat
+  len : Nat
+  dir : Bool
+
+notation "(" start " ..< " stop ")" => Range.mk start (stop - start) false
+notation "(" start " ..≤ " stop ")" => Range.mk start (stop + 1 - start) false
+
+notation "(" start " ..> " stop ")" => Range.mk (stop + 1) (start - stop) true
+notation "(" start " ..≥ " stop ")" => Range.mk stop (start + 1 - stop) true
+
+def Range.rev (range : Range) : Range :=
+  { range with dir := !range.dir }
+
+instance : Membership Nat Range where
+  mem n range := range.start ≤ n ∧ n < range.len + range.start
+
+instance : ForIn m Range Nat where
+  forIn range b f :=
+    let rec forward b i
+      | 0 => return b
+      | l + 1 => do
+        match ← f i b with
+        | .done b => return b
+        | .yield b => forward b (i + 1) l
+    let rec reverse b i
+      | 0 => return b
+      | l + 1 => do
+        match ← f (i + l) b with
+        | .done b => return b
+        | .yield b => reverse b i l
+    match range.dir with
+    | false => forward b range.start range.len
+    | true => reverse b range.start range.len
+
+instance : ForIn' m Range Nat inferInstance where
+  forIn' range b f :=
+    let rec forward b i : ∀ l, range.start ≤ i ∧ i + l ≤ range.len + range.start → _
+      | 0, _ => return b
+      | l + 1, h => do
+        match ← f i ⟨h.1, Nat.le_trans (Nat.succ_le_succ (Nat.le_add_right _ _)) h.2⟩ b with
+        | .done b => return b
+        | .yield b => forward b (i + 1) l ⟨h.1.step, Nat.add_assoc i 1 l ▸ Nat.add_comm 1 l ▸ h.2⟩
+    let rec reverse b : ∀ l, l ≤ range.len → _
+      | 0, _ => return b
+      | l + 1, h => do
+        match ← f (l + range.start) ⟨Nat.le_add_left _ l, Nat.add_lt_add_right h _⟩ b with
+        | .done b => return b
+        | .yield b => reverse b l (Nat.pred_le_pred h.step)
+    match range.dir with
+    | false => forward b range.start range.len ⟨.refl, Nat.add_comm _ _ ▸ .refl⟩
+    | true => reverse b range.len .refl
