sorting/Sorting/Tactic.lean
@@ -1,0 +1,63 @@
+import Lean
+
+open Lean Meta
+
+private def modifyLocalDecl [Monad M] (lctx : LocalContext) (e : Expr) (f : LocalDecl → M LocalDecl) : M LocalContext :=
+  match lctx with
+  | { fvarIdToDecl := map, decls := decls } =>
+    match lctx.findFVar? e with
+    | none      => return lctx
+    | some decl => do
+      let decl ← f decl
+      return { fvarIdToDecl := map.insert decl.fvarId decl
+               decls        := decls.set decl.index decl }
+
+partial def reduceStar (e : Expr) : MetaM Expr :=
+  let rec visit (e : Expr) : MonadCacheT Expr Expr MetaM Expr :=
+    checkCache e fun _ => withIncRecDepth do
+      let e ← whnf e
+      match e with
+      | .app .. =>
+        let f     ← visit e.getAppFn
+        let mut args  := e.getAppArgs
+        for i in [:args.size] do
+          args ← args.modifyM i visit
+        return mkAppN f args
+      | .lam ..        => lambdaTelescope e fun xs b => do
+        let mut lctx ← getLCtx
+        for x in xs do
+          lctx ← modifyLocalDecl lctx x λ e => return e.setType (← visit e.type)
+        withLCtx lctx (← getLocalInstances) do
+          return (← mkLambdaFVars xs (← visit b)).eta
+      | .forallE ..    => forallTelescope e fun xs b => do
+        let mut lctx ← getLCtx
+        for x in xs do
+          lctx ← modifyLocalDecl lctx x λ e => return e.setType (← visit e.type)
+        withLCtx lctx (← getLocalInstances) do
+          mkForallFVars xs (← visit b)
+      | .proj n i s .. => return mkProj n i (← visit s)
+      | _                  => return e
+  withTheReader Core.Context (fun ctx => { ctx with options := ctx.options.setBool `smartUnfolding false }) <|
+    withTransparency .all <|
+      visit e |>.run
+
+open Elab
+
+elab tk:"#reduce*" term:term : command =>
+  withoutModifyingEnv <| Command.runTermElabM fun _ => Term.withDeclName `_reduceStar do
+    let e ← Term.elabTerm term none
+    Term.synthesizeSyntheticMVarsNoPostponing
+    let e ← Term.levelMVarToParam (← instantiateMVars e)
+    logInfoAt tk (← reduceStar e)
+
+syntax "replace " ident (" : " term)? " := " term : tactic
+
+macro_rules
+  | `(tactic| replace $i $[: $t]? := $v) =>
+    `(tactic| have $[: $t]? := $v; clear $i; rename _ => $i)
+
+syntax "split " "with " binderIdent : tactic
+
+macro_rules
+  | `(tactic| split with $i) =>
+    `(tactic| split <;> rename_i $i)
