sorting/Sorting2.lean
@@ -1,0 +1,84 @@
+import Sorting.List
+
+variable (le : α → α → Bool)
+
+def insert (x : α) : List α → List α
+  | [] => [x]
+  | y :: l =>
+    if le x y
+    then x :: y :: l
+    else y :: insert x l
+
+def insertionSort : List α → List α
+  | [] => []
+  | x :: l => insert le x (insertionSort l)
+
+theorem perm_insert x : ∀ l, List.Perm (insert le x l) (x :: l)
+  | [] => .cons x .nil
+  | y :: l => show List.Perm (ite ..) _ from
+    if h : le x y
+    then if_pos h ▸ .cons x (.cons y (.refl l))
+    else if_neg h ▸ .trans (.cons y (perm_insert x l)) (.swap x y (.refl l))
+
+theorem perm_insertionSort : ∀ l, List.Perm (insertionSort le l) l
+  | [] => .nil
+  | x :: l => .trans (perm_insert le x (insertionSort le l)) (.cons x (perm_insertionSort l))
+
+def insertPerm (x : α) : (l : List α) → { r // List.Perm r (x :: l) }
+  | [] => ⟨[x], .cons x .nil⟩
+  | y :: l =>
+    if le x y
+    then ⟨x :: y :: l, .cons x (.cons y (.refl l))⟩
+    else
+      let ⟨r, h⟩ := insertPerm x l
+      ⟨y :: r, .trans (.cons y h) (.swap x y (.refl l))⟩
+
+def insertionSortPerm : (l : List α) → { r // List.Perm r l }
+  | [] => ⟨[], .nil⟩
+  | x :: l =>
+    let ⟨r, h⟩ := insertionSortPerm l
+    let ⟨r', h'⟩ := insertPerm le x r
+    ⟨r', .trans h' (.cons x h)⟩
+
+theorem chain_insert (hle : ∀ {x y}, ¬le x y → le y x) x : ∀ {l}, List.Chain (le · ·) l → List.Chain (le · ·) (insert le x l)
+  | [], _ => .singleton x
+  | y :: l, h => show List.Chain _ (ite ..) from
+    if h' : le x y
+    then if_pos h' ▸ .cons h' h
+    else if_neg h' ▸ match l with
+                     | [] => .cons (hle h') (.singleton x)
+                     | z :: l => show List.Chain _ (_ :: ite ..) from
+                       if h'' : le x z
+                       then if_pos h'' ▸ .cons (hle h') (.cons h'' h.snd)
+                       else if_neg h'' ▸ .cons h.fst (have := if_neg h'' ▸ show List.Chain _ (ite ..) from chain_insert hle x h.snd; by exact this)
+
+variable [Monad m] {α} (le : α → α → m Bool)
+
+def insertM (x : α) : List α → m (List α)
+  | [] => return [x]
+  | y :: l => do
+    if ← le x y
+    then return x :: y :: l
+    else return y :: (← insertM x l)
+
+def insertionSortM : List α → m (List α)
+  | [] => return []
+  | x :: l => do
+    let r ← insertionSortM l
+    insertM le x r
+
+def insertPermM (x : α) : (l : List α) → m { r // List.Perm r (x :: l) }
+  | [] => return ⟨[x], by simp /- .cons x .nil -/⟩
+  | y :: l => do
+    if ← le x y
+    then return ⟨x :: y :: l, .cons x (.cons y (.refl l))⟩
+    else
+      let r ← insertPermM x l
+      return ⟨y :: r.1, .trans (.cons y r.2) (.swap x y (.refl l))⟩
+
+def insertionSortPermM : (l : List α) → m { r // List.Perm r l }
+  | [] => return ⟨[], .nil⟩
+  | x :: l => do
+    let r ← insertionSortPermM l
+    let r' ← insertPermM le x r.1
+    return ⟨r'.1, .trans r'.2 (.cons x r.2)⟩
