sorting/iSorting.lean
@@ -1,0 +1,151 @@
+def LoopT (m : Type u → Type v) (α : Type u) : Type (max (u + 1) v) :=
+  (∀ {β}, (Unit → β → m (ForInStep β)) → β → m β) → m α
+
+instance [Monad m] : Monad (LoopT m) where
+  pure x _ := return x
+  bind f g loop := do g (← f @loop) @loop
+
+instance : ForIn (LoopT m) Lean.Loop Unit where
+  forIn _ b f loop := loop (λ a b => f a b @loop) b
+
+def LoopT.run [Monad m] (f : LoopT m α) : m α :=
+  f Lean.Loop.forIn.loop
+
+def isort [Monad m] (a : List Nat) : LoopT m (List Nat) := do
+  let mut l := a
+  let mut i := l.length - 1
+  while 0 < i do
+    let x := l[i - 1]!
+    let mut j := i
+    while j < a.length do
+      if x ≤ l[j]! then break
+      l := l.set (j - 1) l[j]!
+      j := j + 1
+    l := l.set (j - 1) x
+    i := i - 1
+  return l
+
+def loopFuel : Nat → ∀ {β}, (Unit → β → Option (ForInStep β)) → β → Option β
+  | 0, _, _, _ => none
+  | n + 1, _, f, b => do
+    match ← f () b with
+    | .done b => b
+    | .yield b => loopFuel n f b
+
+#eval isort [5, 4, 3, 2, 1] |>.run |> Id.run
+#eval isort [5, 4, 3, 2, 1] (loopFuel 5)
+
+def Option.get : (o : Option α) → o ≠ none → α
+  | some x, _ => x
+
+theorem Option.get_some (h : o = some x) : Option.get o h' = x := by
+  cases h
+  rfl
+
+theorem loopFuel_monotone : ∀ {n m}, n ≤ m → loopFuel n f b ≠ none → loopFuel m f b ≠ none
+  | _, _, .refl, h => h
+  | _ + 1, _ + 1, hnm, h => by
+    dsimp [loopFuel, bind, Option.bind] at h ⊢
+    split <;> rename_i h' <;> simp [h'] at h ⊢
+    split <;> rename_i h' <;> simp [h'] at h ⊢
+    apply loopFuel_monotone (Nat.pred_le_pred hnm) h
+
+def ForInStep.ok (t : β → Nat) (up : Nat) : ForInStep β → Prop
+  | .done _ => True
+  | .yield b => 0 < t b ∧ t b < up
+
+theorem termination (t : β → Nat) (f : Unit → β → Option (ForInStep β)) (b : β) (init : 0 < t b) (iter : ∀ b, (h : f () b ≠ none) ×' ((f () b).get h).ok t (t b)) : loopFuel (t b) f b ≠ none := by
+  generalize htb : t b = n
+  induction n using Nat.strongInductionOn generalizing b with
+  | _ n ih =>
+  cases htb
+  cases htb : t b with
+  | zero => cases htb ▸ init
+  | succ n =>
+    cases iter b with | _ iter₁ iter₂ =>
+    dsimp [loopFuel, bind, Option.bind]
+    split
+    intro; apply iter₁; assumption
+    dsimp
+    split
+    simp
+    rename_i heq
+    simp [Option.get_some heq, ForInStep.ok] at iter₂
+    apply loopFuel_monotone
+    exact Nat.pred_le_pred (htb ▸ iter₂.right)
+    dsimp
+    apply ih _ iter₂.right _ iter₂.left rfl
+
+example l : ∃ n, isort l (@loopFuel n) ≠ none := by
+  cases l with
+  | nil => exists 1
+  | cons x l =>
+  exists l.length + 1
+  simp only [isort, forIn, pure, bind, Option.bind]
+  split <;> simp
+  rename_i h; revert h
+  show _ ≠ _
+  apply termination (MProd.fst · + 1) _ ⟨_, _⟩ (Nat.zero_lt_succ _)
+  intro b
+  constructor
+  case fst =>
+    split <;> simp
+    split <;> simp
+    rename_i h; revert h
+    show _ ≠ _
+    cases b with | _ b₁ b₂ =>
+    by_cases hb : b₁ < l.length + 1
+    case inr => simp [loopFuel, bind, Option.bind, hb]
+    apply loopFuel_monotone
+    show List.length l + 2 - b₁ ≤ _
+    apply Nat.sub_le_of_le_add
+    rw [Nat.add_assoc, Nat.add_comm 1]
+    apply Nat.add_le_add_left
+    apply Nat.succ_le_succ
+    assumption
+    apply termination (l.length + 2 - MProd.fst ·) _ ⟨_, _⟩
+    simp
+    apply Nat.le_sub_of_add_le
+    rw [Nat.add_comm]
+    apply Nat.le.step
+    exact hb
+    intro b
+    constructor
+    case fst =>
+      split <;> simp
+      split <;> simp
+    case snd =>
+      rename_i h
+      simp [Option.get]
+      dsimp
+      split
+      rename_i h₁ _
+      split at h₁ <;> simp at h₁ <;> simp [← h₁, ForInStep.ok]
+      split at h₁ <;> simp at h₁ <;> simp [← h₁, ForInStep.ok]
+      constructor
+      apply Nat.le_sub_of_add_le
+      rw [Nat.add_comm]
+      apply Nat.succ_le_succ
+      assumption
+      rw [Nat.add_sub_add_right _ 1]
+      apply Nat.le_sub_of_add_le
+      rw [Nat.succ_add]
+      apply Nat.succ_le_succ
+      rw [Nat.sub_add_cancel]
+      exact .refl
+      apply Nat.le_of_lt
+      assumption
+  case snd =>
+    split
+    case inr => simp [Option.get, ForInStep.ok]
+    rename_i h
+    dsimp
+    simp [Option.get]
+    split
+    rename_i h₁ _
+    split at h₁ <;> simp at h₁
+    simp [← h₁, ForInStep.ok]
+    rw [Nat.sub_add_cancel h]
+    constructor
+    exact h
+    exact .refl
